frodo/spec/Spec.Frodo.KEM.Encaps.fst
@@ -24,73 +24,22 @@ val update_ct:
     c1:lbytes (params_logq * params_nbar * params_n / 8)
   -> c2:lbytes (params_logq * params_nbar * params_nbar / 8)
   -> d:lbytes crypto_bytes
-  -> res:lbytes crypto_ciphertextbytes
-    {let c1Len = params_logq * params_nbar * params_n / 8 in
-     let c2Len = params_logq * params_nbar * params_nbar / 8 in
-     expand_crypto_ciphertextbytes ();
-     Seq.sub res 0 c1Len == c1 /\
-     Seq.sub res c1Len c2Len == c2 /\
-     Seq.sub res (c1Len + c2Len) crypto_bytes == d}
-let update_ct c1 c2 d =
-  expand_crypto_ciphertextbytes ();
-  let c1Len = params_logq * params_nbar * params_n / 8 in
-  let c2Len = params_logq * params_nbar * params_nbar / 8 in
-  let ct = Seq.create crypto_ciphertextbytes (u8 0) in
-  let ct = update_sub ct 0 c1Len c1 in
-  let ct = update_sub ct c1Len c2Len c2 in
-  eq_intro (Seq.sub ct 0 c1Len) c1;
-  let ct = update_sub ct (c1Len + c2Len) crypto_bytes d in
-  eq_intro (Seq.sub ct 0 c1Len) c1;
-  eq_intro (Seq.sub ct c1Len c2Len) c2;
-  ct
-
-val lemma_update_ct:
-    c1:lbytes (params_logq * params_nbar * params_n / 8)
-  -> c2:lbytes (params_logq * params_nbar * params_nbar / 8)
-  -> d:lbytes crypto_bytes
-  -> ct:lbytes crypto_ciphertextbytes
-  -> Lemma
-    (requires (
-      let c1Len = params_logq * params_nbar * params_n / 8 in
-      let c2Len = params_logq * params_nbar * params_nbar / 8 in
-      expand_crypto_ciphertextbytes ();
-      Seq.sub ct 0 c1Len == c1 /\
-      Seq.sub ct c1Len c2Len == c2 /\
-      Seq.sub ct (c1Len + c2Len) crypto_bytes == d))
-    (ensures ct == update_ct c1 c2 d)
-let lemma_update_ct c1 c2 d ct =
-  let ct1 = update_ct c1 c2 d in
-  let c1Len = params_logq * params_nbar * params_n / 8 in
-  let c2Len = params_logq * params_nbar * params_nbar / 8 in
-  expand_crypto_ciphertextbytes ();
-
-  FStar.Seq.Properties.lemma_split (Seq.sub ct 0 (c1Len + c2Len)) c1Len;
-  FStar.Seq.Properties.lemma_split (Seq.sub ct1 0 (c1Len + c2Len)) c1Len;
-  FStar.Seq.Properties.lemma_split ct (c1Len + c2Len);
-  FStar.Seq.Properties.lemma_split ct1 (c1Len + c2Len)
+  -> lbytes crypto_ciphertextbytes
+let update_ct c1 c2 d = c1 @| c2 @| d
 
 val update_ss_init:
     c12:lbytes (crypto_ciphertextbytes - crypto_bytes)
   -> kd:lbytes (crypto_bytes + crypto_bytes)
-  -> res:lbytes (crypto_ciphertextbytes + crypto_bytes)
-    {Seq.sub res 0 (crypto_ciphertextbytes - crypto_bytes) == c12 /\
-     Seq.sub res (crypto_ciphertextbytes - crypto_bytes) (crypto_bytes + crypto_bytes) == kd}
-let update_ss_init c12 kd =
-  let ss_init_len = crypto_ciphertextbytes + crypto_bytes in
-  let ss_init = Seq.create ss_init_len (u8 0) in
-  let ss_init = update_sub ss_init 0 (crypto_ciphertextbytes - crypto_bytes) c12 in
-  let ss_init = update_sub ss_init (crypto_ciphertextbytes - crypto_bytes) (crypto_bytes + crypto_bytes) kd in
-  eq_intro (Seq.sub ss_init 0 (crypto_ciphertextbytes - crypto_bytes)) c12;
-  ss_init
+  -> lbytes (crypto_ciphertextbytes + crypto_bytes)
+let update_ss_init c12 kd = c12 @| kd
 
 val update_ss:
     c12:lbytes (crypto_ciphertextbytes - crypto_bytes)
   -> kd:lbytes (crypto_bytes + crypto_bytes)
-  -> res:lbytes crypto_bytes
+  -> lbytes crypto_bytes
 let update_ss c12 kd =
   let ss_init = update_ss_init c12 kd in
-  let ss = frodo_prf_spec (crypto_ciphertextbytes + crypto_bytes) ss_init (u16 7) crypto_bytes in
-  ss
+  frodo_prf_spec (crypto_ciphertextbytes + crypto_bytes) ss_init (u16 7) crypto_bytes
 
 val frodo_mul_add_sa_plus_e:
     seed_a:lbytes bytes_seed_a
