frodo/spec/Spec.Frodo.KEM.KeyGen.fst
@@ -5,13 +5,11 @@ open Lib.Sequence
 open Lib.ByteSequence
 
 open FStar.Mul
-open FStar.Math.Lemmas
 
 open Spec.Matrix
 open Spec.Frodo.Lemmas
 open Spec.Frodo.Params
 open Spec.Frodo.KEM
-open Spec.Frodo.Encode
 open Spec.Frodo.Pack
 open Spec.Frodo.Sample
 
@@ -26,65 +24,15 @@ let crypto_publicmatrixbytes: size_nat =
 val update_pk:
     seed_a:lbytes bytes_seed_a
   -> b:lbytes crypto_publicmatrixbytes
-  -> res:lbytes crypto_publickeybytes
-    {Seq.sub res 0 bytes_seed_a == seed_a /\
-     Seq.sub res bytes_seed_a crypto_publicmatrixbytes == b}
-let update_pk seed_a b =
-  let pk = Seq.create crypto_publickeybytes (u8 0) in
-  let pk = update_sub pk 0 bytes_seed_a seed_a in
-  let pk = update_sub pk bytes_seed_a crypto_publicmatrixbytes b in
-  eq_intro (Seq.sub pk 0 bytes_seed_a) seed_a;
-  pk
-
-val lemma_update_pk:
-    seed_a:lbytes bytes_seed_a
-  -> b:lbytes crypto_publicmatrixbytes
-  -> pk:lbytes crypto_publickeybytes
-  -> Lemma
-    (requires
-      Seq.sub pk 0 bytes_seed_a == seed_a /\
-      Seq.sub pk bytes_seed_a crypto_publicmatrixbytes == b)
-    (ensures pk == update_pk seed_a b)
-let lemma_update_pk seed_a b pk =
-  let pk1 = update_pk seed_a b in
-  FStar.Seq.Properties.lemma_split pk bytes_seed_a;
-  FStar.Seq.Properties.lemma_split pk1 bytes_seed_a
+  -> lbytes crypto_publickeybytes
+let update_pk seed_a b = seed_a @| b
 
 val update_sk:
     s:lbytes crypto_bytes
   -> pk:lbytes crypto_publickeybytes
   -> s_bytes:lbytes (2 * params_n * params_nbar)
-  -> res:lbytes crypto_secretkeybytes
-    {Seq.sub res 0 crypto_bytes == s /\
-     Seq.sub res crypto_bytes crypto_publickeybytes == pk /\
-     Seq.sub res (crypto_bytes + crypto_publickeybytes) (2 * params_n * params_nbar) == s_bytes}
-let update_sk s pk s_bytes =
-  let sk = Seq.create crypto_secretkeybytes (u8 0) in
-  let sk = update_sub sk 0 crypto_bytes s in
-  let sk = update_sub sk crypto_bytes crypto_publickeybytes pk in
-  eq_intro (Seq.sub sk 0 crypto_bytes) s;
-  let sk = update_sub sk (crypto_bytes + crypto_publickeybytes) (2 * params_n * params_nbar) s_bytes in
-  eq_intro (Seq.sub sk 0 crypto_bytes) s;
-  eq_intro (Seq.sub sk crypto_bytes crypto_publickeybytes) pk;
-  sk
-
-val lemma_update_sk:
-    s:lbytes crypto_bytes
-  -> pk:lbytes crypto_publickeybytes
-  -> s_bytes:lbytes (2 * params_n * params_nbar)
-  -> sk:lbytes crypto_secretkeybytes
-  -> Lemma
-    (requires
-      Seq.sub sk 0 crypto_bytes == s /\
-      Seq.sub sk crypto_bytes crypto_publickeybytes == pk /\
-      Seq.sub sk (crypto_bytes + crypto_publickeybytes) (2 * params_n * params_nbar) == s_bytes)
-    (ensures sk == update_sk s pk s_bytes)
-let lemma_update_sk s pk s_bytes sk =
-  let sk1 = update_sk s pk s_bytes in
-  FStar.Seq.Properties.lemma_split (Seq.sub sk 0 (crypto_bytes + crypto_publickeybytes)) crypto_bytes;
-  FStar.Seq.Properties.lemma_split (Seq.sub sk1 0 (crypto_bytes + crypto_publickeybytes)) crypto_bytes;
-  FStar.Seq.Properties.lemma_split sk (crypto_bytes + crypto_publickeybytes);
-  FStar.Seq.Properties.lemma_split sk1 (crypto_bytes + crypto_publickeybytes)
+  -> lbytes crypto_secretkeybytes
+let update_sk s pk s_bytes = s @| pk @| s_bytes
 
 val frodo_mul_add_as_plus_e_pack:
     seed_a:lbytes bytes_seed_a
@@ -119,7 +67,8 @@ let crypto_kem_keypair_ coins =
   let sk = update_sk s pk s_bytes in
   pk, sk
 
-val crypto_kem_keypair: state:Spec.Frodo.Random.state_t
+val crypto_kem_keypair:
+    state:Spec.Frodo.Random.state_t
   -> tuple2 (lbytes crypto_publickeybytes) (lbytes crypto_secretkeybytes)
 let crypto_kem_keypair state =
   let coins, _ = Spec.Frodo.Random.randombytes_ state (2 * crypto_bytes + bytes_seed_a) in
